Clean up the logical relation
Get rid of this typemap bs

theories/examples/various.v
@@ -1,19 +1,20 @@
-(** Examples from Huisman-Worah-Sunesen CSFW-06 *)
+(** Small examples *)
 From iris.base_logic Require Import invariants.
 From iris_ni.logrel Require Import types.
 From iris_ni.program_logic Require Import dwp heap_lang_lifting.
 From iris.proofmode Require Import tactics.
 From iris.heap_lang Require Import lang proofmode.
 From iris_ni.proofmode Require Import dwp_tactics.
-From iris_ni.logrel Require Import typemap interp.
+From iris_ni.logrel Require Import interp.
 From iris_ni.examples Require Import par.
 
+(** Examples from Huisman-Worah-Sunesen CSFW-06 *)
 
 Definition loop : val := rec: "loop" <> := "loop" #().
 Definition t4 : val := λ: "l", ("l" <- #7) ||| (loop #()).
 
-Section proof.
-  Context `{!heapDG Σ, !typemapG (loc*loc) Σ, !spawnG Σ}.
+Section t4_proof.
+  Context `{!heapDG Σ, !spawnG Σ}.
 
   (** According to Huisman's definition of observational determinism
   this program is *not* secure. Because there is a trace that assigns
@@ -22,19 +23,52 @@ Section proof.
   assignment is not executed. Those traces are *not* equivalent up to
   stuttering. *)
   Lemma t4_safe (l1 l2 : val) ξ :
-    locationsI ξ -∗
     ⟦ tref (tint Low) ⟧ ξ l1 l2 -∗
     DWP (t4 l1) & (t4 l2) : ⟦ tprod tunit tunit ⟧ ξ.
   Proof.
-    iIntros "#Hinv #Hl". dwp_rec. dwp_pures.
+    iIntros "#Hl". dwp_rec. dwp_pures.
     iApply (dwp_par (⟦tunit⟧ ξ) (⟦tunit⟧ ξ)).
-    - iApply (interp.dwp_store with "Hinv [Hl]").
+    - iApply (logrel_store with "[Hl]").
       + by iApply dwp_value.
       + iApply dwp_value. iModIntro. iExists _,_. eauto with iFrame.
     - iLöb as "IH". dwp_rec.
       iApply "IH".
-    - iIntros (????) "??".
+    - iIntros (????) "??". rewrite (interp_eq (tprod _ _)).
       iNext. iExists _,_,_,_. eauto with iFrame.
   Qed.
 
-End proof.
+End t4_proof.
+
+(** Awkward exmples *)
+
+(* awk : tint^low → (tunit → τ) → tint^low *)
+Definition awk : val :=
+  λ: "v", let: "x" := ref "v" in
+          λ: "f", "x" <- #1;; "f" #();; !"x".
+
+Section awk_proof.
+  Context `{!heapDG Σ}.
+
+  Definition f_ty τ l : type := tarrow tunit τ l.
+
+  Lemma awk_typing τ l ξ :
+    DWP awk & awk : ⟦ tarrow (tint Low)
+                       (tarrow (f_ty τ l) (tint Low) Low) Low ⟧ ξ.
+  Proof.
+    iApply logrel_lam. iAlways. iIntros (i1 i2) "#Hi". iSimpl.
+    dwp_bind (ref _)%E (ref _)%E. iApply dwp_wand.
+    { iApply logrel_alloc. iApply (dwp_value with "Hi"). }
+    iIntros (r1 r2) "#Hr". dwp_pures.
+    iApply logrel_lam. iAlways.
+    rewrite /f_ty (interp_eq (tarrow _ _ _)). iIntros (f1 f2) "#Hf". iSimpl.
+    dwp_bind (_ <- _)%E (_ <- _)%E. iApply dwp_wand.
+    { iApply logrel_store; first by iApply dwp_value.
+      iApply logrel_int. }
+    iIntros (? ?) "H". iApply (logrel_seq with "[H]").
+    { by iApply dwp_value. }
+    iApply logrel_seq.
+    { iApply "Hf". rewrite (interp_eq tunit). eauto with iFrame. }
+    iApply logrel_deref. rewrite !left_id.
+    iApply (dwp_value with "Hr").
+  Qed.
+End awk_proof.
